src/Testing/LayoutInfoModule.v
@@ -1,0 +1,10 @@
+From StackSafety Require Import MachineModule.
+
+Module Type LayoutInfo (M : Machine).
+  Import M.
+  Parameter LayoutInfo : Type.
+  Parameter defLayoutInfo : LayoutInfo.
+  Parameter defStackMap : LayoutInfo -> StackMap.
+  Parameter CodeMap_Impl : Type.
+  Parameter CodeMap_fromImpl : CodeMap_Impl -> CodeMap.
+End LayoutInfo.
