src/Testing/TestMPC.v
@@ -1,0 +1,19 @@
+From StackSafety Require Import MachineModule PolicyModule TestCtxModule LayoutInfoModule.
+
+From QuickChick Require Import QuickChick.
+
+Module TestMPC (M : Machine) (P : Policy M) (LI : LayoutInfo M) (C : TestCtx M LI).
+  Import M.
+  Import P.
+  Import C.
+  Import LI.
+  
+  Definition MPCState : Type := MachineState * PolicyState * CtxState.
+  Definition mstate : MPCState -> MachineState := fun '(m,p,cs) => m.
+  Definition pstate : MPCState -> PolicyState := fun '(m,p,cs) => p.
+  Definition cstate : MPCState -> CtxState := fun '(m,p,cs) => cs.
+  Definition mpcstep (mpc:MPCState) (cm : CodeMap_Impl) : option (MPCState * Observation) :=
+    option_map
+      (fun '(m,p,o) => (m,p,CtxStateUpdate (mstate mpc) cm (cstate mpc),o))
+      (mpstep (mstate mpc,pstate mpc)).
+End TestMPC.
